Add validity constraint to the `step` type

src/Ouroboros-Mini_Protocols.thy
@@ -16,17 +16,44 @@ record ('s\<^sub>1, 'd\<^sub>1, 's\<^sub>2, 'd\<^sub>2) situation =
 definition dual :: "('s\<^sub>1, 'd\<^sub>1, 's\<^sub>2, 'd\<^sub>2) situation \<Rightarrow> ('s\<^sub>2, 'd\<^sub>2, 's\<^sub>1, 'd\<^sub>1) situation" where
   [simp]: "dual situation = \<lparr>state = sum_swap (state situation), data = prod.swap (data situation)\<rparr>"
 
-record ('s\<^sub>a, 'd\<^sub>a, 's\<^sub>p, 'd\<^sub>p, 'm) steps =
+record ('s\<^sub>a, 'd\<^sub>a, 's\<^sub>p, 'd\<^sub>p, 'm) unchecked_steps =
   initiation :: "'s\<^sub>a \<Rightarrow> 'd\<^sub>a \<Rightarrow> ('m \<times> 'd\<^sub>a) successor"
   completion :: "'m \<Rightarrow> 's\<^sub>a \<rightharpoonup> ('s\<^sub>a + 's\<^sub>p) \<times> ('d\<^sub>p \<Rightarrow> 'd\<^sub>p)"
 
+definition unchecked_steps_are_valid :: "('s\<^sub>a, 'd\<^sub>a, 's\<^sub>p, 'd\<^sub>p, 'm) unchecked_steps \<Rightarrow> bool" where
+  [simp]: "unchecked_steps_are_valid \<S> =
+    (\<forall>s\<^sub>a d\<^sub>a m d\<^sub>a'. initiation \<S> s\<^sub>a d\<^sub>a = Continuing (m, d\<^sub>a') \<longrightarrow> s\<^sub>a \<in> dom (completion \<S> m))"
+
 definition
-  step :: "('s\<^sub>a, 'd\<^sub>a, 's\<^sub>p, 'd\<^sub>p, 'm) steps \<Rightarrow> 's\<^sub>a \<Rightarrow> 'd\<^sub>a \<times> 'd\<^sub>p \<Rightarrow> ('s\<^sub>a, 'd\<^sub>a, 's\<^sub>p, 'd\<^sub>p) situation successor"
+  unchecked_step :: "
+    ('s\<^sub>a, 'd\<^sub>a, 's\<^sub>p, 'd\<^sub>p, 'm) unchecked_steps \<Rightarrow>
+    's\<^sub>a \<Rightarrow>
+    'd\<^sub>a \<times> 'd\<^sub>p \<Rightarrow>
+    ('s\<^sub>a, 'd\<^sub>a, 's\<^sub>p, 'd\<^sub>p) situation successor"
 where
-  [simp]: "step \<S> s\<^sub>a d =
+  [simp]: "unchecked_step \<S> s\<^sub>a d =
     map_successor
       (\<lambda>(m, d\<^sub>a'). let (s', D) = the (completion \<S> m s\<^sub>a) in \<lparr>state = s', data = (d\<^sub>a', D (snd d))\<rparr>)
       (initiation \<S> s\<^sub>a (fst d))"
+
+typedef ('s\<^sub>a, 'd\<^sub>a, 's\<^sub>p, 'd\<^sub>p, 'm) steps =
+  "{\<S> :: ('s\<^sub>a, 'd\<^sub>a, 's\<^sub>p, 'd\<^sub>p, 'm) unchecked_steps. unchecked_steps_are_valid \<S>}"
+proof -
+  have "unchecked_steps_are_valid \<lparr>initiation = \<lambda>_ _. Done, completion = \<lambda>_ _. None\<rparr>"
+    by simp
+  then show ?thesis
+    by blast
+qed
+
+setup_lifting type_definition_steps
+
+lift_definition
+  step :: "
+    ('s\<^sub>a, 'd\<^sub>a, 's\<^sub>p, 'd\<^sub>p, 'm) steps \<Rightarrow>
+    's\<^sub>a \<Rightarrow>
+    'd\<^sub>a \<times> 'd\<^sub>p \<Rightarrow>
+    ('s\<^sub>a, 'd\<^sub>a, 's\<^sub>p, 'd\<^sub>p) situation successor"
+  is unchecked_step .
 
 record ('s\<^sub>c, 'd\<^sub>c, 's\<^sub>s, 'd\<^sub>s, 'm) transitions =
   client_steps :: "('s\<^sub>c, 'd\<^sub>c, 's\<^sub>s, 'd\<^sub>s, 'm) steps"
